# baseURI: file:/C:/Users/cox075/dev/ontologies/trunk/O&M-OWL/PROV_SSN.ttl

@prefix dc: <http://purl.org/dc/elements/1.1/> .
@prefix dul: <http://www.loa-cnr.it/ontologies/DUL.owl#> .
@prefix owl: <http://www.w3.org/2002/07/owl#> .
@prefix prov: <http://www.w3.org/ns/prov#> .
@prefix prov_ssn: <http://purl.oclc.org/NET/ssnprov/ssnprov#> .
@prefix rdf: <http://www.w3.org/1999/02/22-rdf-syntax-ns#> .
@prefix rdfs: <http://www.w3.org/2000/01/rdf-schema#> .
@prefix ssn: <http://purl.oclc.org/NET/ssnx/ssn#> .
@prefix xml: <http://www.w3.org/XML/1998/namespace> .
@prefix xsd: <http://www.w3.org/2001/XMLSchema#> .

<file:///C:/Users/cox075/dev/ontologies/trunk/O&M-OWL/PROV_SSN.ttl>
  rdf:type owl:Ontology ;
  rdfs:comment """Converted from http://purl.oclc.org/NET/ssnprov/ssnprov (which redirects to https://raw.githubusercontent.com/dcorsar/ssnprov/master/PROV_SSN.rdf )

A number of errors fixed:
1. no namespace binding for prefix dc:
2. incorrect URI for PROV-O
3. add an explicit namespace prefix for prov_ssn:"""^^xsd:string ;
.
<http://purl.oclc.org/NET/ssnprov/ssnprov>
  rdf:type owl:Ontology ;
  dc:creator "David Corsar"^^xsd:string ;
  dc:creator "Kerry Taylor"^^xsd:string ;
  dc:creator "Michael Compton"^^xsd:string ;
  rdfs:comment "This ontology describes an alignment of the W3C Semantic Sensor Network (SSN( Incubator Group's SSN Ontology and the W3C Provenance Working Group's PROV-O ontoloyg.  The alignment extends the expressive capability of the SSNO for recording observations and system deployments, enabling more comprehensive historical information to be described than is possible using SSNO alone."^^xsd:string ;
.
prov_ssn:ActivityOfSensing
  rdf:type owl:Class ;
  rdfs:comment "The prov:Activity of a ssn:Sensor performing the sensing.  An ActivityOfSensing prov:generated the ssn:SensorOutput,  was influenced by (prov:wasInfluencedBy) the ssn:Stimulus and, through SensorPerformedSensing (a prov:Association), prov:wasAssociatedWith the sensor."^^xsd:string ;
  rdfs:subClassOf prov:Activity ;
  rdfs:subClassOf [
      rdf:type owl:Restriction ;
      owl:onProperty prov:generated ;
      owl:someValuesFrom ssn:SensorOutput ;
    ] ;
  rdfs:subClassOf [
      rdf:type owl:Restriction ;
      owl:onProperty prov:qualifiedAssociation ;
      owl:someValuesFrom prov_ssn:SensorPerformedSensing ;
    ] ;
  rdfs:subClassOf [
      rdf:type owl:Restriction ;
      owl:onProperty prov:qualifiedUsage ;
      owl:someValuesFrom prov_ssn:SensingUsage ;
    ] ;
  rdfs:subClassOf [
      rdf:type owl:Restriction ;
      owl:onProperty prov:wasInfluencedBy ;
      owl:someValuesFrom ssn:Stimulus ;
    ] ;
.
prov_ssn:ObservationInterpretation
  rdf:type owl:Class ;
  rdfs:comment """
The prov:Activity of ObservationInterpretation records the activity that interpreted the results of an ActivityOfSensing and resulted in (prov:generated) a dul:Situation that is the ssn:Observation.  The activity of ObservationInterpretation prov:wasInformedBy the ActivityOfSensing and may be prov:wasInformedBy some of the aspects recorded by the ssn:Observation.
         """^^xsd:string ;
  rdfs:subClassOf prov:Activity ;
  rdfs:subClassOf [
      rdf:type owl:Restriction ;
      owl:onProperty prov:generated ;
      owl:someValuesFrom ssn:Observation ;
    ] ;
  rdfs:subClassOf [
      rdf:type owl:Restriction ;
      owl:onProperty prov:wasInformedBy ;
      owl:someValuesFrom prov_ssn:ActivityOfSensing ;
    ] ;
.
prov_ssn:PerformedSensing
  rdf:type owl:Class ;
  rdfs:comment """
         The prov:Role of a ssn:Sensor in a SensorPerformedSensing that is prov:qualifiedAssociation with an ActivityOfSensing. 
         """^^xsd:string ;
  rdfs:subClassOf prov:Role ;
.
prov_ssn:SensingMethod
  rdf:type owl:Class ;
  rdfs:comment """
         The prov:Role of ssn:Sensing in a SensorUsage that is prov:qualifiedUsage with an ActivityOfSensing. 
         """^^xsd:string ;
  rdfs:subClassOf prov:Role ;
.
prov_ssn:SensingUsage
  rdf:type owl:Class ;
  rdfs:comment """
         The  of a ssn:Sensing for an ActivityOfSensing. 
         The ActivityOfSensing prov:qualifiedUsage for describing the prov:Role and prov:Plan used by a ssn:Sensor when performing sensing.
       
         """^^xsd:string ;
  rdfs:subClassOf prov:Usage ;
  rdfs:subClassOf [
      rdf:type owl:Restriction ;
      owl:onProperty prov:entity ;
      owl:someValuesFrom ssn:Sensing ;
    ] ;
  rdfs:subClassOf [
      rdf:type owl:Restriction ;
      owl:onProperty prov:hadRole ;
      owl:someValuesFrom prov_ssn:SensingMethod ;
    ] ;
.
prov_ssn:SensorPerformedSensing
  rdf:type owl:Class ;
  rdfs:comment """
         The ActivityOfSensing prov:qualifiedAssociation for describing the prov:Role and prov:Plan followed by a ssn:Sensor when performing sensing. 
         """^^xsd:string ;
  rdfs:subClassOf prov:Association ;
  rdfs:subClassOf [
      rdf:type owl:Restriction ;
      owl:onProperty prov_ssn:sensingAgent ;
      owl:someValuesFrom ssn:Sensor ;
    ] ;
  rdfs:subClassOf [
      rdf:type owl:Restriction ;
      owl:onProperty prov:hadPlan ;
      owl:someValuesFrom ssn:Sensing ;
    ] ;
  rdfs:subClassOf [
      rdf:type owl:Restriction ;
      owl:onProperty prov:hadRole ;
      owl:someValuesFrom prov_ssn:PerformedSensing ;
    ] ;
.
prov_ssn:sensingAgent
  rdf:type owl:ObjectProperty ;
  rdfs:subPropertyOf prov:agent ;
  owl:inverseOf prov_ssn:sensingAgentINV ;
.
prov_ssn:sensingAgentINV
  rdf:type owl:ObjectProperty ;
.
ssn:DeploymentRelatedProcess
  rdfs:subClassOf prov:Activity ;
.
ssn:Observation
  rdfs:subClassOf prov:Entity ;
.
ssn:ObservationValue
  rdfs:subClassOf prov:Entity ;
  rdfs:subClassOf [
      rdf:type owl:Restriction ;
      owl:onProperty prov:alternateOf ;
      owl:someValuesFrom ssn:SensorOutput ;
    ] ;
.
ssn:Platform
  rdfs:subClassOf prov:Entity ;
.
ssn:Sensing
  rdfs:subClassOf prov:Plan ;
.
ssn:Sensor
  rdfs:subClassOf prov:Agent ;
  rdfs:subClassOf prov:Entity ;
.
ssn:SensorOutput
  rdfs:subClassOf prov:Entity ;
  rdfs:subClassOf [
      rdf:type owl:Restriction ;
      owl:onProperty prov:alternateOf ;
      owl:someValuesFrom ssn:ObservationValue ;
    ] ;
.
ssn:Stimulus
  rdfs:subClassOf prov:Activity ;
.
ssn:System
  rdfs:subClassOf prov:Collection ;
.
ssn:deployedOnPlatform
  rdfs:subPropertyOf prov:used ;
.
ssn:deployedSystem
  rdfs:subPropertyOf prov:used ;
.
ssn:hasSubSystem
  rdfs:subPropertyOf prov:hadMember ;
.
ssn:implements
  owl:propertyChainAxiom (
      prov_ssn:sensingAgentINV
      prov:hadPlan
    ) ;
.
ssn:isProducedBy
  rdfs:subPropertyOf prov:wasAttributedTo ;
.
ssn:observationResult
  rdfs:subPropertyOf prov:wasDerivedFrom ;
.
ssn:observedBy
  rdfs:subPropertyOf prov:wasAttributedTo ;
.
